chore(BKS): Add Helper functions to select KMS Encryption Context for HV-2

AwsCryptographicMaterialProviders/dafny/AwsCryptographyKeyStore/src/Structure.dfy
@@ -132,6 +132,17 @@ module {:options "/functionSyntax:4" } Structure {
         || BRANCH_KEY_TYPE_PREFIX < m[TYPE_FIELD])
   }
 
+  predicate Hv2EncryptionContext?(m: map<string, string>) {
+    && (BRANCH_KEY_IDENTIFIER_FIELD !in m)
+    && (TYPE_FIELD !in m)
+    && (KEY_CREATE_TIME !in m)
+    && (HIERARCHY_VERSION !in m)
+    && (TABLE_FIELD !in m)
+    && (KMS_FIELD !in m)
+    && (BRANCH_KEY_FIELD !in m.Keys)
+    && (BRANCH_KEY_ACTIVE_VERSION_FIELD !in m)
+  }
+
   predicate EncryptedHierarchicalKey?(key: Types.EncryptedHierarchicalKey) {
     && BranchKeyContext?(key.EncryptionContext)
     && key.Identifier == key.EncryptionContext[BRANCH_KEY_IDENTIFIER_FIELD]
